Add Char.some to basis
This commit adds the following function to the Char module:

    Char.some: char -> char option

The Char.some function returns its char argument wrapped in a Some
constructor. It does so *without* performing on-the-fly allocation;
instead it looks up the returned value from a pre-computed vector.

The implementation is written in a way that makes this code easily
dead-code eliminated if it is unused. Thus the pre-computed vector
should only be present in memory if it is actually used.

This function is meant to be used in TextIO.

basis/CharProgScript.sml
@@ -27,16 +27,43 @@ val _ = trans ">=" stringSyntax.char_ge_tm;
 val _ = next_ml_names := ["isSpace"];
 val res = translate stringTheory.isSpace_def;
 
-val sigs = module_signatures [
-  "ord",
-  "chr",
-  "<",
-  ">",
-  "<=",
-  ">=",
-  "isSpace"
-];
+Definition some_chars_vector_def:
+  some_chars_vector = Vector (GENLIST (λn. SOME (CHR n)) 256)
+End
 
-val _ = ml_prog_update (close_module (SOME sigs));
+Definition some_char_def:
+  some_char c = regexp_compiler$sub some_chars_vector (ORD c)
+End
+
+Theorem some_char_thm:
+  some_char c = SOME c
+Proof
+  Cases_on ‘c’
+  \\ rewrite_tac [some_chars_vector_def,some_char_def,regexp_compilerTheory.sub_def]
+  \\ full_simp_tac std_ss [ORD_CHR]
+  \\ full_simp_tac std_ss [GSYM ORD_CHR]
+  \\ full_simp_tac std_ss [EL_GENLIST]
+QED
+
+val _ = ml_prog_update open_local_block;
+
+val res = translate (EVAL “some_chars_vector”);
+
+val _ = ml_prog_update open_local_in_block;
+
+val _ = next_ml_names := ["some"];
+val res = translate some_char_def;
+
+Triviality some_char_side_thm:
+  some_char_side v = T
+Proof
+  fs [fetch "-" "some_char_side_def"] \\ EVAL_TAC \\ fs [ORD_BOUND]
+QED
+
+val _ = update_precondition some_char_side_thm;
+
+val _ = ml_prog_update close_local_blocks;
+
+val _ = ml_prog_update (close_module NONE);
 
 val _ = export_theory()
